work at the assert level whenever possible

veric/Clight_seplog.v
@@ -37,26 +37,17 @@ Section mpred.
 
 Context `{!heapGS Σ}.
 
-Definition var_block (sh: Share.t) {cs: compspecs} (idt: ident * type) (rho: environ): mpred :=
+Local Notation assert := (@assert Σ).
+
+Definition var_block (sh: Share.t) {cs: compspecs} (idt: ident * type): assert :=
   ⌜sizeof (snd idt) <= Ptrofs.max_unsigned⌝ ∧
-  (memory_block sh (sizeof (snd idt))) (eval_lvar (fst idt) (snd idt) rho).
+  assert_of (fun rho => (memory_block sh (sizeof (snd idt))) (eval_lvar (fst idt) (snd idt) rho)).
 
-Definition stackframe_of {cs: compspecs} (f: Clight.function) : environ -> mpred :=
-  fold_right (fun P Q rho => P rho ∗ Q rho) (fun rho => emp) (map (fun idt => var_block Share.top idt) (Clight.fn_vars f)).
+Definition stackframe_of {cs: compspecs} (f: Clight.function) : assert :=
+  fold_right bi_sep emp (map (fun idt => var_block Share.top idt) (Clight.fn_vars f)).
 
-Lemma stackframe_of_eq : forall {cs: compspecs}, stackframe_of =
-        fun f rho => fold_right bi_sep emp (map (fun idt => var_block Share.top idt rho) (Clight.fn_vars f)).
-Proof.
-  intros.
-  extensionality f rho.
-  unfold stackframe_of.
-  forget (fn_vars f) as vl.
-  induction vl; simpl; auto.
-  rewrite IHvl; auto.
-Qed.
-
-Lemma  subst_derives:
- forall a v (P Q : environ -> mpred), (forall rho, P rho ⊢ Q rho) -> forall rho, subst a v P rho ⊢ subst a v Q rho.
+Lemma subst_derives:
+ forall a v (P Q : assert), (P ⊢ Q) -> assert_of (subst a v P) ⊢ assert_of (subst a v Q).
 Proof.
   exact subst_extens.
 Qed.
@@ -67,21 +58,21 @@ Definition tc_formals (formals: list (ident * type)) : environ -> Prop :=
 (*This definition, and some lemmas below, could be moved to general_seplog*)
 
 Definition close_precondition (bodyparams: list ident) 
-    (P: argsEnviron -> mpred) (rho:environ) : mpred :=
- ∃ vals,
+    (P: argsassert) : assert :=
+ assert_of (fun rho => ∃ vals,
    ⌜map (Map.get (te_of rho)) bodyparams = map Some vals /\
       Forall (fun v : val => v <> Vundef) vals⌝ ∧
-   P (ge_of rho, vals).
+   P (ge_of rho, vals)).
 
 Definition precondition_closed (fs: list (ident*type)) {A}
-  (P: A -> environ -> mpred) : Prop :=
+  (P: A -> assert) : Prop :=
  forall x,
   closed_wrt_vars (not_a_param fs) (P x) /\
   closed_wrt_lvars (fun _ => True%type) (P x).
 
 Lemma close_precondition_e':
-   forall al (P: argsEnviron -> mpred) (rho: environ),
-   close_precondition al P rho ⊢ 
+   forall al (P: argsassert) (rho: environ),
+   close_precondition al P rho ⊢
    ∃ vals,
      ⌜map (Map.get (te_of rho)) al = map Some vals /\
         Forall (fun v : val => v <> Vundef) vals⌝ ∧
@@ -109,11 +100,11 @@ Proof.
 unfold close_precondition.
 apply bi.exist_proper; intros vals; apply bi.and_proper; last done; apply bi.pure_proper; intuition;
   apply (Forall_eval_id_get); trivial.
-Qed. 
+Qed.
 
-Definition bind_args (bodyparams: list (ident * type)) (P: genviron * list val -> mpred) : environ -> mpred :=
-  fun rho => ⌜tc_formals bodyparams rho⌝
-     ∧ close_precondition (map fst bodyparams) P rho.
+Definition bind_args (bodyparams: list (ident * type)) (P: argsassert) : assert :=
+  local (tc_formals bodyparams)
+     ∧ close_precondition (map fst bodyparams) P.
 
 Definition ret_temp : ident := 1%positive.
 
@@ -126,13 +117,13 @@ Definition get_result (ret: option ident) : environ -> environ :=
  | Some x => get_result1 x
  end.
 
-Definition bind_ret (vl: option val) (t: type) (Q: environ -> mpred) : environ -> mpred :=
-     match vl, t with
-     | None, Tvoid => fun rho => Q (make_args nil nil rho)
-     | Some v, _ => fun rho => ⌜tc_val t v⌝ ∧
+Definition bind_ret (vl: option val) (t: type) (Q: assert) : assert :=
+     assert_of (fun rho => match vl, t with
+     | None, Tvoid => Q (make_args nil nil rho)
+     | Some v, _ => ⌜tc_val t v⌝ ∧
                                Q (make_args (ret_temp::nil) (v::nil) rho)
-     | _, _ => fun rho => False
-     end.
+     | _, _ => False
+     end).
 
 Definition funassert (Delta: tycontext): assert := funspecs_assert (glob_specs Delta).
 
@@ -150,10 +141,10 @@ Definition proj_ret_assert (Q: @ret_assert Σ) (ek: exitkind) (vl: option val) :
  | EK_return => RA_return Q vl
  end.
 
-Definition overridePost  (Q: environ -> mpred)  (R: ret_assert) :=
+Definition overridePost  (Q: assert)  (R: ret_assert) :=
  match R with 
   {| RA_normal := _; RA_break := b; RA_continue := c; RA_return := r |} =>
-  {| RA_normal := assert_of Q; RA_break := b; RA_continue := c; RA_return := r |}
+  {| RA_normal := Q; RA_break := b; RA_continue := c; RA_return := r |}
  end.
 
 Definition existential_ret_assert {A: Type} (R: A -> @ret_assert Σ) :=
@@ -163,25 +154,25 @@ Definition existential_ret_assert {A: Type} (R: A -> @ret_assert Σ) :=
      RA_return := fun vl => ∃ x:A, (R x).(RA_return) vl
    |}.
 
-Definition normal_ret_assert (Q: environ -> mpred) : ret_assert :=
-  {| RA_normal := assert_of Q; RA_break := False; RA_continue := False; RA_return := fun _ => False |}.
+Definition normal_ret_assert (Q: assert) : ret_assert :=
+  {| RA_normal := Q; RA_break := False; RA_continue := False; RA_return := fun _ => False |}.
 
-Definition frame_ret_assert (R: ret_assert) (F: environ -> mpred) : ret_assert :=
+Definition frame_ret_assert (R: ret_assert) (F: assert) : ret_assert :=
  match R with 
   {| RA_normal := n; RA_break := b; RA_continue := c; RA_return := r |} =>
-  {| RA_normal := n ∗ assert_of F;
-     RA_break := b ∗ assert_of F;
-     RA_continue := c ∗ assert_of F;
-     RA_return := fun vl => r vl ∗ assert_of F |}
+  {| RA_normal := n ∗ F;
+     RA_break := b ∗ F;
+     RA_continue := c ∗ F;
+     RA_return := fun vl => r vl ∗ F |}
  end.
 
-Definition conj_ret_assert (R: ret_assert) (F: environ -> mpred) : ret_assert :=
+Definition conj_ret_assert (R: ret_assert) (F: assert) : ret_assert :=
  match R with 
   {| RA_normal := n; RA_break := b; RA_continue := c; RA_return := r |} =>
-  {| RA_normal := n ∧ assert_of F;
-     RA_break := b ∧ assert_of F;
-     RA_continue := c ∧ assert_of F;
-     RA_return := fun vl => r vl ∧ assert_of F |}
+  {| RA_normal := n ∧ F;
+     RA_break := b ∧ F;
+     RA_continue := c ∧ F;
+     RA_return := fun vl => r vl ∧ F |}
  end.
 
 Definition switch_ret_assert (R: @ret_assert Σ) : ret_assert :=
@@ -194,23 +185,21 @@ Definition switch_ret_assert (R: @ret_assert Σ) : ret_assert :=
  end.
 
 Lemma normal_ret_assert_derives:
- forall P Q rho,
-  (P rho ⊢ Q rho) ->
-  forall ek vl, proj_ret_assert (normal_ret_assert P) ek vl rho
-            ⊢ proj_ret_assert (normal_ret_assert Q) ek vl rho.
+ forall P Q,
+  (P ⊢ Q) ->
+  forall ek vl, proj_ret_assert (normal_ret_assert P) ek vl
+            ⊢ proj_ret_assert (normal_ret_assert Q) ek vl.
 Proof.
   intros.
   destruct ek; simpl; auto.
-  rewrite !monPred_at_and /= H //.
+  rewrite H //.
 Qed.
 
 Lemma normal_ret_assert_False:
-  forall ek vl, proj_ret_assert (normal_ret_assert (False : assert)) ek vl ⊣⊢ False.
+  forall ek vl, proj_ret_assert (normal_ret_assert False) ek vl ⊣⊢ False.
 Proof.
 intros.
-destruct ek; simpl; auto; try by rewrite bi.and_False.
-split => ?.
-rewrite monPred_at_and /= monPred_pure_unfold !monPred_at_embed /= bi.and_False //.
+destruct ek; simpl; auto; by rewrite bi.and_False.
 Qed.
 
 (* Do we care about the kind of equivalence? Should this be an assert? *)
@@ -220,15 +209,14 @@ Global Instance ret_assert_equiv : Equiv (@ret_assert Σ) := fun a b =>
 
 Lemma frame_normal:
   forall P F,
-   ret_assert_equiv (frame_ret_assert (normal_ret_assert P) F) (normal_ret_assert (fun rho => P rho ∗ F rho)).
+   ret_assert_equiv (frame_ret_assert (normal_ret_assert P) F) (normal_ret_assert (P ∗ F)).
 Proof.
 intros.
 unfold normal_ret_assert; simpl.
-split3; last split; simpl; auto; intros; rewrite ?bi.sep_False //.
-split => ?; rewrite monPred_at_sep //.
+split3; last split; simpl; auto; intros; rewrite bi.sep_False //.
 Qed.
 
-Lemma pure_and_sep_assoc: forall P (Q R : mpred), ⌜P⌝ ∧ Q ∗ R ⊣⊢ (⌜P⌝ ∧ Q) ∗ R.
+Lemma pure_and_sep_assoc: forall {PROP} P (Q R : bi_car PROP), ⌜P⌝ ∧ Q ∗ R ⊣⊢ (⌜P⌝ ∧ Q) ∗ R.
 Proof.
   intros; iSplit.
   - iIntros "($ & $ & $)".
@@ -236,38 +224,36 @@ Proof.
 Qed.
 
 Lemma proj_frame:
-  forall P F ek vl rho,
-    proj_ret_assert (frame_ret_assert P F) ek vl rho ⊣⊢ F rho ∗ proj_ret_assert P ek vl rho.
+  forall P F ek vl,
+    proj_ret_assert (frame_ret_assert P F) ek vl ⊣⊢ F ∗ proj_ret_assert P ek vl.
 Proof.
   intros.
   rewrite bi.sep_comm.
-  destruct ek; simpl; destruct P; rewrite /= ?monPred_at_and monPred_at_sep //
-    monPred_pure_unfold monPred_at_embed pure_and_sep_assoc //.
+  destruct ek; simpl; destruct P; rewrite ?pure_and_sep_assoc //.
 Qed.
 
 Lemma proj_conj:
-  forall P F ek vl rho,
-    proj_ret_assert (conj_ret_assert P F) ek vl rho ⊣⊢ F rho ∧ proj_ret_assert P ek vl rho.
+  forall P F ek vl,
+    proj_ret_assert (conj_ret_assert P F) ek vl ⊣⊢ F ∧ proj_ret_assert P ek vl.
 Proof.
   intros.
   rewrite bi.and_comm.
-  destruct ek; simpl; destruct P; rewrite /= !monPred_at_and //
-    monPred_pure_unfold monPred_at_embed assoc //.
+  destruct ek; simpl; destruct P; rewrite /= ?assoc //.
 Qed.
 
-Definition loop1_ret_assert (Inv: environ -> mpred) (R: ret_assert) : ret_assert :=
+Definition loop1_ret_assert (Inv: assert) (R: ret_assert) : ret_assert :=
  match R with 
   {| RA_normal := n; RA_break := b; RA_continue := c; RA_return := r |} =>
-  {| RA_normal := assert_of Inv;
+  {| RA_normal := Inv;
      RA_break := n; 
-     RA_continue := assert_of Inv;
+     RA_continue := Inv;
      RA_return := r |}
  end.
 
-Definition loop2_ret_assert (Inv: environ -> mpred) (R: ret_assert) : ret_assert :=
+Definition loop2_ret_assert (Inv: assert) (R: ret_assert) : ret_assert :=
  match R with 
   {| RA_normal := n; RA_break := b; RA_continue := c; RA_return := r |} =>
-  {| RA_normal := assert_of Inv;
+  {| RA_normal := Inv;
      RA_break := n;
      RA_continue := False;
      RA_return := r |}
@@ -275,21 +261,20 @@ Definition loop2_ret_assert (Inv: environ -> mpred) (R: ret_assert) : ret_assert
 
 Lemma frame_for1:
   forall Q R F,
-   (frame_ret_assert (loop1_ret_assert Q R) F ≡
-    loop1_ret_assert (fun rho => Q rho ∗ F rho) (frame_ret_assert R F))%stdpp.
+   (frame_ret_assert (loop1_ret_assert Q R) F =
+    loop1_ret_assert (Q ∗ F) (frame_ret_assert R F))%stdpp.
 Proof.
 intros.
-destruct R; split3; last split; try done; split => ? /=; rewrite monPred_at_sep //.
+destruct R; reflexivity.
 Qed.
 
 Lemma frame_loop1:
   forall Q R F,
-   ret_assert_equiv (frame_ret_assert (loop2_ret_assert Q R) F)
-   (loop2_ret_assert (fun rho => Q rho ∗ F rho) (frame_ret_assert R F)).
+   (frame_ret_assert (loop2_ret_assert Q R) F ≡
+    loop2_ret_assert (Q ∗ F) (frame_ret_assert R F))%stdpp.
 Proof.
-intros.
-destruct R; split3; last split; try done; split => ? /=; rewrite monPred_at_sep //.
-rewrite monPred_pure_unfold monPred_at_embed bi.sep_False //.
+destruct R; split3; last split; try done; simpl.
+apply bi.sep_False.
 Qed.
 
 Lemma overridePost_normal:
@@ -299,11 +284,11 @@ intros; unfold overridePost, normal_ret_assert.
 f_equal.
 Qed.
 
-Definition function_body_ret_assert (ret: type) (Q: environ -> mpred) : ret_assert :=
- {| RA_normal := assert_of (bind_ret None ret Q);
+Definition function_body_ret_assert (ret: type) (Q: assert) : ret_assert :=
+ {| RA_normal := bind_ret None ret Q;
     RA_break := False; 
     RA_continue := False;
-    RA_return := fun vl => assert_of (bind_ret vl ret Q) |}.
+    RA_return := fun vl => bind_ret vl ret Q |}.
 
 Lemma same_glob_funassert:
   forall Delta1 Delta2,
@@ -314,5 +299,5 @@ Proof. intros; apply @same_FS_funspecs_assert; trivial. Qed.
 End mpred.
 
 #[export] Hint Resolve normal_ret_assert_derives : core.
-(*#[export] Hint Rewrite normal_ret_assert_False frame_normal frame_for1 frame_loop1
-                 overridePost_normal: normalize.*)
+#[export] Hint Rewrite @normal_ret_assert_False @frame_normal @frame_for1 @frame_loop1
+                 @overridePost_normal: normalize.
