veric/semax_conseq.v
@@ -23,30 +23,29 @@ Require Import VST.veric.Clight_lemmas.
 
 (* Part 1: Proof of semax_conseq *)
 
-Local Notation assert := (environ -> mpred).
-
 Section mpred.
 
-Context `{!heapGS Σ} {Espec : OracleKind} `{!externalGS (@OK_ty Σ Espec) Σ}. (* consolidate *)
+Context `{!heapGS Σ} {Espec : OracleKind} `{!externalGS (@OK_ty Σ Espec) Σ}. (* consolidate? *)
 
 Lemma _guard_mono: forall ge E Delta f (P Q: assert) k,
-  (forall rho, P rho ⊢ Q rho) ->
+  (P ⊢ Q) ->
   _guard Espec ge E Delta f Q k ⊢ _guard Espec ge E Delta f P k.
+Proof.
+  intros.
+  apply _guard_mono; auto.
+  intros; apply H.
+Qed.
+
+Lemma guard_mono: forall ge E Delta f (P Q: assert) k,
+  (P ⊢ Q) ->
+  guard' Espec ge E Delta f Q k ⊢ guard' Espec ge E Delta f P k.
 Proof.
   intros.
   apply _guard_mono; auto.
 Qed.
 
-Lemma guard_mono: forall ge E Delta f (P Q: assert) k,
-  (forall rho, P rho ⊢ Q rho) ->
-  guard' Espec ge E Delta f Q k ⊢ guard' Espec ge E Delta f P k.
-Proof.
-  intros.
-  apply guard_mono; auto.
-Qed.
-
 Lemma rguard_mono: forall ge E Delta f (P Q: ret_assert) k,
-  (forall rk vl rho, proj_ret_assert P rk vl rho ⊢ proj_ret_assert Q rk vl rho) ->
+  (forall rk vl, proj_ret_assert P rk vl ⊢ proj_ret_assert Q rk vl) ->
   rguard Espec ge E Delta f Q k ⊢ rguard Espec ge E Delta f P k.
 Proof.
   intros.
@@ -65,26 +64,25 @@ Definition fupd_ret_assert E (Q: ret_assert): ret_assert :=
    probably add a bupd if we really want to, but it may not be
    necessary. *)
 
-Lemma fupd_fupd_andp_prop : forall E P (Q : mpred), (|={E}=> (⌜P⌝ ∧ |={E}=> Q)) ⊣⊢ (|={E}=> (⌜P⌝ ∧ Q)).
+Lemma fupd_fupd_andp_prop : forall E P (Q : assert), (|={E}=> (⌜P⌝ ∧ |={E}=> Q)) ⊣⊢ (|={E}=> (⌜P⌝ ∧ Q)).
 Proof.
   intros; iSplit; iIntros "H".
   - iMod "H" as "[$ $]".
   - iMod "H" as "[$ $]"; done.
 Qed.
 
-Lemma proj_fupd_ret_assert: forall E Q ek vl rho,
-  (|={E}=> proj_ret_assert (fupd_ret_assert E Q) ek vl rho) ⊣⊢ (|={E}=> proj_ret_assert Q ek vl rho).
+Lemma proj_fupd_ret_assert: forall E Q ek vl,
+  (|={E}=> proj_ret_assert (fupd_ret_assert E Q) ek vl) ⊣⊢ (|={E}=> proj_ret_assert Q ek vl).
 Proof.
   intros.
-  destruct ek; rewrite // /=; monPred.unseal; apply fupd_fupd_andp_prop.
+  destruct ek; rewrite // /=; apply fupd_fupd_andp_prop.
 Qed.
 
-(* The following four lemmas are not now used. but after deep embedded hoare logic (SL_as_Logic) is
-ported, the frame does not need to be quantified in the semantic definition of semax. Then,
-these two lemmas can replace the other two afterwards. *)
+(* After deep embedded hoare logic (SL_as_Logic) is ported, maybe the frame does not need to be
+   quantified in the semantic definition of semax. *)
 
 Lemma assert_safe_fupd':
-  forall gx vx tx rho E (P: environ -> mpred) Delta f k,
+  forall gx vx tx E (P: assert) Delta f k rho,
     match k with Ret _ _ => False | _ => True end ->
     let PP1 := ⌜guard_environ Delta f rho⌝ in
     let PP2 := funassert Delta rho in
@@ -99,20 +97,21 @@ Proof.
 Qed.
 
 Lemma _guard_fupd':
-  forall ge E Delta (P: environ -> mpred) f k,
+  forall ge E Delta (P: assert) f k,
     match k with Ret _ _ => False | _ => True end ->
-    _guard Espec ge E Delta f P k ⊣⊢ _guard Espec ge E Delta f (fun rho => |={E}=> (P rho)) k.
+    _guard Espec ge E Delta f P k ⊣⊢ _guard Espec ge E Delta f (|={E}=> P) k.
 Proof.
   intros.
   unfold _guard.
   apply bi.forall_proper; intros ?.
   apply bi.forall_proper; intros ?.
   rewrite assert_safe_fupd'; auto.
+  by monPred.unseal.
 Qed.
 
 Lemma guard_fupd':
-  forall ge E Delta f (P: environ -> mpred) k,
-    guard' Espec ge E Delta f P k ⊣⊢ guard' Espec ge E Delta f (fun rho => |={E}=> (P rho)) k.
+  forall ge E Delta f (P: assert) k,
+    guard' Espec ge E Delta f P k ⊣⊢ guard' Espec ge E Delta f (|={E}=> P) k.
 Proof.
   intros.
   apply _guard_fupd'; auto.
@@ -142,28 +141,29 @@ Proof.
 Qed.
 
 Lemma assert_safe_fupd:
-  forall gx vx tx rho E (F P: environ -> mpred) Delta f k,
+  forall gx vx tx rho E (F P: assert) Delta f k,
     match k with Ret _ _ => False | _ => True end ->
     let PP1 := ⌜guard_environ Delta f rho⌝ in
     let PP2 := funassert Delta rho in
-    (PP1 ∧ (F rho ∗ P rho) ∗ PP2 -∗
+    (PP1 ∧ (F ∗ P) rho ∗ PP2 -∗
     assert_safe Espec gx E f vx tx k rho) ⊣⊢
-    (PP1 ∧ (F rho ∗ |={E}=> (P rho)) ∗ PP2 -∗
+    (PP1 ∧ (F ∗ |={E}=> P) rho ∗ PP2 -∗
     assert_safe Espec gx E f vx tx k rho).
 Proof.
   intros.
   iSplit.
   * iIntros "H (% & P & #?)".
-    rewrite (assert_safe_fupd' _ _ _ _ _ (fun rho => F rho ∗ P rho)); last done.
-    iPoseProof (fupd_frame_l with "P") as "P".
-    iApply "H"; auto.
-  * iIntros "H (% & (? & P) & ?)"; iApply "H"; iFrame; auto.
+    rewrite (assert_safe_fupd' _ _ _ _ (F ∗ P)); last done.
+    iApply "H"; iFrame "#"; iFrame "%".
+    monPred.unseal; by iDestruct "P" as "($ & >$)".
+  * iIntros "H (% & P & ?)"; iApply "H"; iFrame.
+    iFrame "%"; monPred.unseal; by iDestruct "P" as "($ & $)".
 Qed.
 
 Lemma _guard_fupd:
-  forall ge E Delta f (F P: environ -> mpred) k,
+  forall ge E Delta f (F P: assert) k,
     match k with Ret _ _ => False | _ => True end ->
-    _guard Espec ge E Delta f (fun rho => F rho ∗ P rho) k ⊣⊢ _guard Espec ge E Delta f (fun rho => F rho ∗ |={E}=> (P rho)) k.
+    _guard Espec ge E Delta f (F ∗ P) k ⊣⊢ _guard Espec ge E Delta f (F ∗ |={E}=> P) k.
 Proof.
   intros.
   unfold _guard.
@@ -173,30 +173,29 @@ Proof.
 Qed.
 
 Lemma guard_fupd:
-  forall ge E Delta f (F P: environ -> mpred) k,
-    guard' Espec ge E Delta f (fun rho => F rho ∗ P rho) k ⊣⊢ guard' Espec ge E Delta f (fun rho => F rho ∗ |={E}=> (P rho)) k.
+  forall ge E Delta f (F P: assert) k,
+    guard' Espec ge E Delta f (F ∗ P) k ⊣⊢ guard' Espec ge E Delta f (F ∗ |={E}=> P) k.
 Proof.
   intros.
   apply _guard_fupd; auto.
 Qed.
 
-Lemma fupd_fupd_frame_l : forall E (P Q : mpred), (|={E}=> (P ∗ |={E}=> Q)) ⊣⊢ |={E}=> (P ∗ Q).
+Lemma fupd_fupd_frame_l : forall E (P Q : assert), (|={E}=> (P ∗ |={E}=> Q)) ⊣⊢ |={E}=> (P ∗ Q).
 Proof.
   intros; iSplit.
   - by iIntros ">[$ >$]".
   - by iIntros ">[$ $]".
 Qed.
 
-Lemma proj_fupd_ret_assert_frame: forall E F Q ek vl rho,
-  (|={E}=> (F ∗ proj_ret_assert (fupd_ret_assert E Q) ek vl rho)) ⊣⊢ |={E}=> (F ∗ proj_ret_assert Q ek vl rho).
+Lemma proj_fupd_ret_assert_frame: forall E F Q ek vl,
+  (|={E}=> (F ∗ proj_ret_assert (fupd_ret_assert E Q) ek vl)) ⊣⊢ |={E}=> (F ∗ proj_ret_assert Q ek vl).
 Proof.
   intros.
-  destruct ek; simpl; auto; monPred.unseal;
+  destruct ek; simpl; auto;
     rewrite -fupd_fupd_frame_l fupd_fupd_andp_prop fupd_fupd_frame_l; auto.
 Qed.
 
-(* this would be unnecessary if assert worked properly *)
-Global Instance guard_proper ge E Delta f : Proper ((fun a b => forall rho, a rho ⊣⊢ b rho) ==> eq ==> equiv) (_guard Espec ge E Delta f).
+Global Instance guard_proper ge E Delta f : Proper (equiv ==> eq ==> equiv) (_guard Espec ge E Delta f).
 Proof.
   intros ????? ->; rewrite /_guard.
   do 7 f_equiv.
@@ -205,10 +204,9 @@ Qed.
 
 Lemma guard_proj_frame : forall ge E Delta f P F ek vl k,
   _guard Espec ge E Delta f (proj_ret_assert (frame_ret_assert P F) ek vl) k ⊣⊢
-  _guard Espec ge E Delta f (fun rho => F rho ∗ proj_ret_assert P ek vl rho) k.
+  _guard Espec ge E Delta f (F ∗ proj_ret_assert P ek vl) k.
 Proof.
-  intros; apply guard_proper; last done.
-  intros; by rewrite proj_frame.
+  intros. rewrite proj_frame //.
 Qed.
 
 Lemma rguard_fupd:
@@ -227,30 +225,32 @@ Proof.
 Qed.
 
 Lemma _guard_allp_fun_id:
-  forall ge E Delta' Delta f (F P: environ -> mpred) k,
+  forall ge E Delta' Delta f (F P: assert) k,
     tycontext_sub E Delta Delta' ->
-    _guard Espec ge E Delta' f (fun rho => F rho ∗ P rho) k ⊣⊢ _guard Espec ge E Delta' f (fun rho => F rho ∗ (<affine> allp_fun_id E Delta rho ∗ P rho)) k.
+    _guard Espec ge E Delta' f (F ∗ P) k ⊣⊢ _guard Espec ge E Delta' f (F ∗ (<affine> allp_fun_id E Delta ∗ P)) k.
 Proof.
   intros.
   unfold _guard.
   do 7 f_equiv.
   iSplit.
-  * iIntros "(($ & $) & #f)".
-    by iPoseProof (funassert_allp_fun_id_sub with "f") as "$".
-  * iIntros "(($ & _ & $) & $)".
+  * monPred.unseal; rewrite monPred_at_affinely.
+    iIntros "(($ & $) & f)"; iSplit; last done.
+    by iIntros "!>"; iApply funassert_allp_fun_id_sub.
+  * monPred.unseal.
+    iIntros "(($ & _ & $) & $)".
 Qed.
 
-Lemma guard_allp_fun_id: forall ge E Delta' Delta f (F P: environ -> mpred) k,
+Lemma guard_allp_fun_id: forall ge E Delta' Delta f (F P: assert) k,
   tycontext_sub E Delta Delta' ->
-  guard' Espec ge E Delta' f (fun rho => F rho ∗ P rho) k ⊣⊢ guard' Espec ge E Delta' f (fun rho => F rho ∗ (<affine> allp_fun_id E Delta rho ∗ P rho)) k.
+  guard' Espec ge E Delta' f (F ∗ P) k ⊣⊢ guard' Espec ge E Delta' f (F ∗ (<affine> allp_fun_id E Delta ∗ P)) k.
 Proof.
   intros.
   apply _guard_allp_fun_id; auto.
 Qed.
 
-Lemma rguard_allp_fun_id: forall ge E Delta' Delta f (F: environ -> mpred) P k,
+Lemma rguard_allp_fun_id: forall ge E Delta' Delta f (F: assert) P k,
   tycontext_sub E Delta Delta' ->
-  rguard Espec ge E Delta' f (frame_ret_assert P F) k ⊣⊢ rguard Espec ge E Delta' f (frame_ret_assert (frame_ret_assert P (fun rho => <affine> allp_fun_id E Delta rho)) F) k.
+  rguard Espec ge E Delta' f (frame_ret_assert P F) k ⊣⊢ rguard Espec ge E Delta' f (frame_ret_assert (frame_ret_assert P (<affine> allp_fun_id E Delta)) F) k.
 Proof.
   intros.
   unfold rguard.
@@ -263,32 +263,32 @@ Proof.
 Qed.
 
 Lemma _guard_tc_environ:
-  forall ge E Delta' Delta f (F P: environ -> mpred) k,
+  forall ge E Delta' Delta f (F P: assert) k,
     tycontext_sub E Delta Delta' ->
-    _guard Espec ge E Delta' f (fun rho => F rho ∗ P rho) k ⊣⊢
-    _guard Espec ge E Delta' f (fun rho => F rho ∗ (⌜typecheck_environ Delta rho⌝ ∧ P rho)) k.
+    _guard Espec ge E Delta' f (F ∗ P) k ⊣⊢
+    _guard Espec ge E Delta' f (F ∗ (local (typecheck_environ Delta) ∧ P)) k.
 Proof.
   intros.
   unfold _guard.
   do 6 f_equiv.
   iSplit.
-  * iIntros "(%Henv & ($ & $) & $)"; iPureIntro.
+  * monPred.unseal; iIntros "(%Henv & ($ & $) & $)"; iPureIntro.
     split3; auto; eapply typecheck_environ_sub; eauto.
     destruct Henv as [? _]; auto.
-  * iIntros "($ & ($ & [_ $]) & $)".
+  * monPred.unseal; iIntros "($ & ($ & [_ $]) & $)".
 Qed.
 
-Lemma guard_tc_environ: forall ge E Delta' Delta f (F P: environ -> mpred) k,
+Lemma guard_tc_environ: forall ge E Delta' Delta f (F P: assert) k,
   tycontext_sub E Delta Delta' ->
-  guard' Espec ge E Delta' f (fun rho => F rho ∗ P rho) k ⊣⊢ guard' Espec ge E Delta' f (fun rho => F rho ∗ (⌜typecheck_environ Delta rho⌝ ∧ P rho)) k.
+  guard' Espec ge E Delta' f (F ∗ P) k ⊣⊢ guard' Espec ge E Delta' f (F ∗ (local (typecheck_environ Delta) ∧ P)) k.
 Proof.
   intros.
   apply _guard_tc_environ; auto.
 Qed.
 
-Lemma rguard_tc_environ: forall ge E Delta' Delta f (F: environ -> mpred) P k,
+Lemma rguard_tc_environ: forall ge E Delta' Delta f (F: assert) P k,
   tycontext_sub E Delta Delta' ->
-  rguard Espec ge E Delta' f (frame_ret_assert P F) k ⊣⊢ rguard Espec ge E Delta' f (frame_ret_assert (conj_ret_assert P (fun rho => ⌜typecheck_environ Delta rho⌝)) F) k.
+  rguard Espec ge E Delta' f (frame_ret_assert P F) k ⊣⊢ rguard Espec ge E Delta' f (frame_ret_assert (conj_ret_assert P (local (typecheck_environ Delta))) F) k.
 Proof.
   intros.
   unfold rguard.
@@ -299,18 +299,28 @@ Proof.
   intros; by rewrite proj_conj.
 Qed.
 
+Global Instance local_absorbing l : Absorbing (@local Σ l).
+Proof.
+  rewrite /local; apply monPred_absorbing, _.
+Qed.
+
+Global Instance local_persistent l : Persistent (@local Σ l).
+Proof.
+  rewrite /local; apply monPred_persistent, _.
+Qed.
+
 Lemma semax'_conseq {CS: compspecs}:
  forall E Delta P' (R': ret_assert) P c (R: ret_assert) ,
-   (forall rho, ⌜typecheck_environ Delta rho⌝ ∧ (<affine> allp_fun_id E Delta rho ∗ P rho) ⊢
-                   (|={E}=> (P' rho)) ) ->
-   (forall rho,  ⌜typecheck_environ Delta rho⌝ ∧ (<affine> allp_fun_id E Delta rho ∗ RA_normal R' rho) ⊢
-                   (|={E}=> (RA_normal R rho))) ->
-   (forall rho, ⌜typecheck_environ Delta rho⌝ ∧ (<affine> allp_fun_id E Delta rho ∗ RA_break R' rho) ⊢
-                   (|={E}=> (RA_break R rho))) ->
-   (forall rho, ⌜typecheck_environ Delta rho⌝ ∧ (<affine> allp_fun_id E Delta rho ∗ RA_continue R' rho) ⊢
-                   (|={E}=> (RA_continue R rho))) ->
-   (forall vl rho, ⌜typecheck_environ Delta rho⌝ ∧ (<affine> allp_fun_id E Delta rho ∗ RA_return R' vl rho) ⊢
-                   (RA_return R vl rho)) ->
+   (local (typecheck_environ Delta) ∧ (<affine> allp_fun_id E Delta ∗ P) ⊢
+                   (|={E}=> P')) ->
+   (local (typecheck_environ Delta) ∧ (<affine> allp_fun_id E Delta ∗ RA_normal R') ⊢
+                   (|={E}=> RA_normal R)) ->
+   (local (typecheck_environ Delta) ∧ (<affine> allp_fun_id E Delta ∗ RA_break R') ⊢
+                   (|={E}=> RA_break R)) ->
+   (local (typecheck_environ Delta) ∧ (<affine> allp_fun_id E Delta ∗ RA_continue R') ⊢
+                   (|={E}=> RA_continue R)) ->
+   (forall vl, local (typecheck_environ Delta) ∧ (<affine> allp_fun_id E Delta ∗ RA_return R' vl) ⊢
+                   RA_return R vl) ->
    semax' Espec E Delta P' c R' ⊢ semax' Espec E Delta P c R.
 Proof.
   intros.
@@ -333,27 +343,26 @@ Proof.
          | rename H1 into Hx; pose (ek:=@RA_break Σ)
          | rename H2 into Hx ; pose (ek:=@RA_continue Σ)
          | apply bi.sep_mono, H3; auto]; clear H3.
-    all: monPred.unseal; rewrite -Hx; iIntros "($ & $ & $ & $ & $)".
+    all: rewrite -Hx; iIntros "($ & $ & $ & $)".
   + erewrite (guard_allp_fun_id _ _ _ _ _ _ P) by eauto.
-    erewrite (guard_tc_environ _ _ _ _ _ _ (fun rho => <affine> allp_fun_id E Delta rho ∗ P rho)) by eauto.
+    erewrite (guard_tc_environ _ _ _ _ _ _ (<affine> allp_fun_id E Delta ∗ P)) by eauto.
     rewrite (guard_fupd _ _ _ _ _ P').
     iApply (guard_mono with "H").
-    intros.
     by rewrite -H.
 Qed.
 
 Lemma semax_conseq {CS: compspecs}:
  forall E Delta P' (R': ret_assert) P c (R: ret_assert) ,
-   (forall rho, ⌜typecheck_environ Delta rho⌝ ∧ (<affine> allp_fun_id E Delta rho ∗ P rho) ⊢
-                   (|={E}=> (P' rho)) ) ->
-   (forall rho,  ⌜typecheck_environ Delta rho⌝ ∧ (<affine> allp_fun_id E Delta rho ∗ RA_normal R' rho) ⊢
-                   (|={E}=> (RA_normal R rho))) ->
-   (forall rho, ⌜typecheck_environ Delta rho⌝ ∧ (<affine> allp_fun_id E Delta rho ∗ RA_break R' rho) ⊢
-                   (|={E}=> (RA_break R rho))) ->
-   (forall rho, ⌜typecheck_environ Delta rho⌝ ∧ (<affine> allp_fun_id E Delta rho ∗ RA_continue R' rho) ⊢
-                   (|={E}=> (RA_continue R rho))) ->
-   (forall vl rho, ⌜typecheck_environ Delta rho⌝ ∧ (<affine> allp_fun_id E Delta rho ∗ RA_return R' vl rho) ⊢
-                   (RA_return R vl rho)) ->
+   (local (typecheck_environ Delta) ∧ (<affine> allp_fun_id E Delta ∗ P) ⊢
+                   (|={E}=> P') ) ->
+   (local (typecheck_environ Delta) ∧ (<affine> allp_fun_id E Delta ∗ RA_normal R') ⊢
+                   (|={E}=> RA_normal R)) ->
+   (local (typecheck_environ Delta) ∧ (<affine> allp_fun_id E Delta ∗ RA_break R') ⊢
+                   (|={E}=> RA_break R)) ->
+   (local (typecheck_environ Delta) ∧ (<affine> allp_fun_id E Delta ∗ RA_continue R') ⊢
+                   (|={E}=> RA_continue R)) ->
+   (forall vl, local (typecheck_environ Delta) ∧ (<affine> allp_fun_id E Delta ∗ RA_return R' vl) ⊢
+                   RA_return R vl) ->
    semax Espec E Delta P' c R' ->  semax Espec E Delta P c R.
 Proof.
   intros.
@@ -363,32 +372,32 @@ Qed.
 (* Part 2: Deriving simpler and older version of consequence rules from semax_conseq. *)
 Lemma semax'_post_fupd:
  forall {CS: compspecs} (R': ret_assert) E Delta (R: ret_assert) P c,
-   (forall ek vl rho, ek <> EK_return -> ⌜typecheck_environ Delta rho⌝ ∧ 
-                proj_ret_assert R' ek vl rho
-         ⊢ |={E}=> (proj_ret_assert R ek vl rho)) ->
-   (forall vl rho,  ⌜typecheck_environ Delta rho⌝ ∧
-                RA_return R' vl rho 
-         ⊢ RA_return R vl rho) ->
+   (forall ek vl, ek <> EK_return -> local (typecheck_environ Delta) ∧
+                proj_ret_assert R' ek vl
+         ⊢ |={E}=> proj_ret_assert R ek vl) ->
+   (forall vl, local (typecheck_environ Delta) ∧
+                RA_return R' vl
+         ⊢ RA_return R vl) ->
    semax' Espec E Delta P c R' ⊢ semax' Espec E Delta P c R.
 Proof.
 intros.
-apply semax'_conseq; [by iIntros (?) "(_ & _ & $)" | .. | intros; rewrite -H0; iIntros "($ & _ & $)"]; intros.
-- specialize (H EK_normal None rho); simpl in H.
+apply semax'_conseq; [by iIntros "(_ & _ & $)" | .. | intros; rewrite -H0; iIntros "($ & _ & $)"]; intros.
+- specialize (H EK_normal None); simpl in H.
   rewrite (bi.pure_True (None = None)) in H; last done; rewrite !bi.True_and in H.
   rewrite -H; last done; iIntros "($ & _ & $)".
-- specialize (H EK_break None rho); simpl in H.
+- specialize (H EK_break None); simpl in H.
   rewrite (bi.pure_True (None = None)) in H; last done; rewrite !bi.True_and in H.
   rewrite -H; last done; iIntros "($ & _ & $)".
-- specialize (H EK_continue None rho); simpl in H.
+- specialize (H EK_continue None); simpl in H.
   rewrite (bi.pure_True (None = None)) in H; last done; rewrite !bi.True_and in H.
   rewrite -H; last done; iIntros "($ & _ & $)".
 Qed.
 
 Lemma semax'_post:
  forall {CS: compspecs} (R': ret_assert) E Delta (R: ret_assert) P c,
-   (forall ek vl rho,  ⌜typecheck_environ Delta rho⌝ ∧ 
-                proj_ret_assert R' ek vl rho 
-         ⊢ proj_ret_assert R ek vl rho) ->
+   (forall ek vl, local (typecheck_environ Delta) ∧
+                proj_ret_assert R' ek vl
+         ⊢ proj_ret_assert R ek vl) ->
    semax' Espec E Delta P c R' ⊢ semax' Espec E Delta P c R.
 Proof.
 intros.
@@ -398,17 +407,17 @@ apply semax'_post_fupd.
 Qed.
 
 Lemma semax'_pre_fupd:
- forall {CS: compspecs} P' E Delta R P c,
+ forall {CS: compspecs} (P' : assert) E Delta R (P : assert) c,
   (forall rho, typecheck_environ Delta rho -> P rho ⊢ |={E}=> (P' rho)) -> 
   semax' Espec E Delta P' c R ⊢ semax' Espec E Delta P c R.
 Proof.
 intros.
 apply semax'_conseq; intros; [| by iIntros "(_ & _ & $)"..].
-iIntros "(% & _ & ?)"; iApply H; auto.
+split => ?; monPred.unseal; iIntros "(% & _ & ?)"; iApply H; auto.
 Qed.
 
 Lemma semax'_pre:
- forall {CS: compspecs} P' E Delta R P c,
+ forall {CS: compspecs} (P': assert) E Delta R (P: assert) c,
   (forall rho, typecheck_environ Delta rho -> P rho ⊢ P' rho) ->
   semax' Espec E Delta P' c R ⊢ semax' Espec E Delta P c R.
 Proof.
@@ -418,14 +427,14 @@ Qed.
 
 Lemma semax'_pre_post_fupd:
  forall
-      {CS: compspecs} P' (R': ret_assert) E Delta (R: ret_assert) P c,
+      {CS: compspecs} (P' : assert) (R': ret_assert) E Delta (R: ret_assert) (P: assert) c,
    (forall rho, typecheck_environ Delta rho -> P rho ⊢ |={E}=> (P' rho)) ->
-   (forall ek vl rho, ek <> EK_return -> ⌜typecheck_environ Delta rho⌝
-                       ∧  proj_ret_assert R ek vl rho 
-                    ⊢ |={E}=> (proj_ret_assert R' ek vl rho)) ->
-   (forall vl rho, ⌜typecheck_environ Delta rho⌝ 
-                       ∧  RA_return R vl rho 
-                    ⊢ RA_return R' vl rho) ->
+   (forall ek vl, ek <> EK_return -> local (typecheck_environ Delta)
+                       ∧  proj_ret_assert R ek vl
+                    ⊢ |={E}=> proj_ret_assert R' ek vl) ->
+   (forall vl, local (typecheck_environ Delta)
+                       ∧  RA_return R vl
+                    ⊢ RA_return R' vl) ->
    semax' Espec E Delta P' c R ⊢ semax' Espec E Delta P c R'.
 Proof.
 intros.
@@ -435,11 +444,11 @@ Qed.
 
 Lemma semax'_pre_post:
  forall
-      {CS: compspecs} P' (R': ret_assert) E Delta (R: ret_assert) P c,
+      {CS: compspecs} (P': assert) (R': ret_assert) E Delta (R: ret_assert) (P: assert) c,
    (forall rho, typecheck_environ Delta rho -> P rho ⊢ P' rho) ->
-   (forall ek vl rho, ⌜typecheck_environ Delta rho⌝
-                       ∧  proj_ret_assert R ek vl rho
-                    ⊢ proj_ret_assert R' ek vl rho) ->
+   (forall ek vl, local (typecheck_environ Delta)
+                       ∧  proj_ret_assert R ek vl
+                    ⊢ proj_ret_assert R' ek vl) ->
    semax' Espec E Delta P' c R ⊢ semax' Espec E Delta P c R'.
 Proof.
 intros.
@@ -449,12 +458,12 @@ Qed.
 
 Lemma semax_post'_fupd {CS: compspecs}:
  forall (R': ret_assert) E Delta (R: ret_assert) P c,
-   (forall ek vl rho, ek <> EK_return -> ⌜typecheck_environ Delta rho⌝ 
-                      ∧  proj_ret_assert R' ek vl rho
-                        ⊢ |={E}=> (proj_ret_assert R ek vl rho)) ->
-   (forall vl rho,  ⌜typecheck_environ Delta rho⌝ 
-                      ∧  RA_return R' vl rho
-                        ⊢ RA_return R vl rho) ->
+   (forall ek vl, ek <> EK_return -> local (typecheck_environ Delta)
+                      ∧  proj_ret_assert R' ek vl
+                        ⊢ |={E}=> proj_ret_assert R ek vl) ->
+   (forall vl, local (typecheck_environ Delta)
+                      ∧  RA_return R' vl
+                        ⊢ RA_return R vl) ->
    semax Espec E Delta P c R' ->  semax Espec E Delta P c R.
 Proof.
 unfold semax.
@@ -464,28 +473,28 @@ Qed.
 
 Lemma semax_post_fupd {CS: compspecs}:
  forall (R': ret_assert) E Delta (R: ret_assert) P c,
-   (forall rho,  ⌜typecheck_environ Delta rho⌝
-                      ∧  RA_normal R' rho ⊢ |={E}=> (RA_normal R rho)) ->
-   (forall rho, ⌜typecheck_environ Delta rho⌝
-                      ∧ RA_break R' rho ⊢ |={E}=> (RA_break R rho)) ->
-   (forall rho, ⌜typecheck_environ Delta rho⌝
-                      ∧ RA_continue R' rho ⊢ |={E}=> (RA_continue R rho)) ->
-   (forall vl rho, ⌜typecheck_environ Delta rho⌝
-                      ∧ RA_return R' vl rho ⊢ RA_return R vl rho) ->
+   (local (typecheck_environ Delta)
+                      ∧  RA_normal R' ⊢ |={E}=> RA_normal R) ->
+   (local (typecheck_environ Delta)
+                      ∧ RA_break R' ⊢ |={E}=> RA_break R) ->
+   (local (typecheck_environ Delta)
+                      ∧ RA_continue R' ⊢ |={E}=> RA_continue R) ->
+   (forall vl, local (typecheck_environ Delta)
+                      ∧ RA_return R' vl ⊢ RA_return R vl) ->
    semax Espec E Delta P c R' ->  semax Espec E Delta P c R.
 Proof.
 unfold semax.
 intros.
 rewrite -semax'_post_fupd; auto.
-destruct ek; try contradiction; intros; simpl; monPred.unseal;
-  iIntros "(% & -> & ?)"; rewrite -> bi.pure_True by done; rewrite bi.True_and; [rewrite -H | rewrite -H0 | rewrite -H1]; auto.
+destruct ek; try contradiction; intros; simpl;
+  iIntros "(? & -> & ?)"; rewrite -> bi.pure_True by done; rewrite bi.True_and; [rewrite -H | rewrite -H0 | rewrite -H1]; auto.
 Qed.
 
 Lemma semax_post' {CS: compspecs}:
  forall (R': ret_assert) E Delta (R: ret_assert) P c,
-   (forall ek vl rho,  ⌜typecheck_environ Delta rho⌝ 
-                      ∧  proj_ret_assert R' ek vl rho
-                        ⊢ proj_ret_assert R ek vl rho) ->
+   (forall ek vl, local (typecheck_environ Delta)
+                      ∧  proj_ret_assert R' ek vl
+                        ⊢ proj_ret_assert R ek vl) ->
    semax Espec E Delta P c R' ->  semax Espec E Delta P c R.
 Proof.
 unfold semax.
@@ -495,56 +504,56 @@ Qed.
 
 Lemma semax_post {CS: compspecs}:
  forall (R': ret_assert) E Delta (R: ret_assert) P c,
-   (forall rho,  ⌜typecheck_environ Delta rho⌝
-                      ∧  RA_normal R' rho ⊢ RA_normal R rho) ->
-   (forall rho, ⌜typecheck_environ Delta rho⌝
-                      ∧ RA_break R' rho ⊢ RA_break R rho) ->
-   (forall rho, ⌜typecheck_environ Delta rho⌝
-                      ∧ RA_continue R' rho ⊢ RA_continue R rho) ->
-   (forall vl rho, ⌜typecheck_environ Delta rho⌝
-                      ∧ RA_return R' vl rho ⊢ RA_return R vl rho) ->
+   (local (typecheck_environ Delta)
+                      ∧  RA_normal R' ⊢ RA_normal R) ->
+   (local (typecheck_environ Delta)
+                      ∧ RA_break R' ⊢ RA_break R) ->
+   (local (typecheck_environ Delta)
+                      ∧ RA_continue R' ⊢ RA_continue R) ->
+   (forall vl, local (typecheck_environ Delta)
+                      ∧ RA_return R' vl ⊢ RA_return R vl) ->
    semax Espec E Delta P c R' ->  semax Espec E Delta P c R.
 Proof.
 unfold semax.
 intros.
 rewrite -semax'_post; auto.
-destruct ek; simpl; auto; intros; monPred.unseal;
-  iIntros "(% & -> & ?)"; rewrite -> bi.pure_True by done; rewrite bi.True_and; [rewrite -H | rewrite -H0 | rewrite -H1]; auto.
+destruct ek; simpl; auto; intros;
+  iIntros "(? & -> & ?)"; rewrite -> bi.pure_True by done; rewrite bi.True_and; [rewrite -H | rewrite -H0 | rewrite -H1]; auto.
 Qed.
 
 Lemma semax_pre_fupd {CS: compspecs} :
  forall P' E Delta P c R,
-   (forall rho, ⌜typecheck_environ Delta rho⌝ ∧  P rho ⊢ |={E}=> (P' rho)) ->
+   (local (typecheck_environ Delta) ∧ P ⊢ |={E}=> P') ->
      semax Espec E Delta P' c R  -> semax Espec E Delta P c R.
 Proof.
 unfold semax.
 intros.
 rewrite -semax'_pre_fupd; auto.
-intros; rewrite -H; auto.
+intros; inversion H as [H']. revert H'; monPred.unseal; intros <-; auto.
 Qed.
 
 Lemma semax_pre {CS: compspecs} :
  forall P' E Delta P c R,
-   (forall rho, ⌜typecheck_environ Delta rho⌝ ∧ P rho ⊢ P' rho) ->
+   (local (typecheck_environ Delta) ∧ P ⊢ P') ->
      semax Espec E Delta P' c R  -> semax Espec E Delta P c R.
 Proof.
 unfold semax.
 intros.
 rewrite -semax'_pre; auto.
-intros; rewrite -H; auto.
+intros; inversion H as [H']; revert H'; monPred.unseal; intros <-; auto.
 Qed.
 
 Lemma semax_pre_post_fupd {CS: compspecs}:
  forall P' (R': ret_assert) E Delta P c (R: ret_assert) ,
-   (forall rho,  ⌜typecheck_environ Delta rho⌝ ∧  P rho ⊢ |={E}=> P' rho) ->
-   (forall rho,  ⌜typecheck_environ Delta rho⌝
-                      ∧  RA_normal R' rho ⊢ |={E}=> (RA_normal R rho)) ->
-   (forall rho, ⌜typecheck_environ Delta rho⌝
-                      ∧ RA_break R' rho ⊢ |={E}=> (RA_break R rho)) ->
-   (forall rho, ⌜typecheck_environ Delta rho⌝
-                      ∧ RA_continue R' rho ⊢ |={E}=> (RA_continue R rho)) ->
-   (forall vl rho, ⌜typecheck_environ Delta rho⌝
-                      ∧ RA_return R' vl rho ⊢ RA_return R vl rho) ->
+   (local (typecheck_environ Delta) ∧ P ⊢ |={E}=> P') ->
+   (local (typecheck_environ Delta)
+                      ∧  RA_normal R' ⊢ |={E}=> RA_normal R) ->
+   (local (typecheck_environ Delta)
+                      ∧ RA_break R' ⊢ |={E}=> RA_break R) ->
+   (local (typecheck_environ Delta)
+                      ∧ RA_continue R' ⊢ |={E}=> RA_continue R) ->
+   (forall vl, local (typecheck_environ Delta)
+                      ∧ RA_return R' vl ⊢ RA_return R vl) ->
    semax Espec E Delta P' c R' ->  semax Espec E Delta P c R.
 Proof.
 intros.
@@ -554,15 +563,15 @@ Qed.
 
 Lemma semax_pre_post {CS: compspecs}:
  forall P' (R': ret_assert) E Delta P c (R: ret_assert) ,
-   (forall rho,  ⌜typecheck_environ Delta rho⌝ ∧ P rho ⊢ P' rho) ->
-   (forall rho,  ⌜typecheck_environ Delta rho⌝
-                      ∧  RA_normal R' rho ⊢ RA_normal R rho) ->
-   (forall rho, ⌜typecheck_environ Delta rho⌝
-                      ∧ RA_break R' rho ⊢ RA_break R rho) ->
-   (forall rho, ⌜typecheck_environ Delta rho⌝
-                      ∧ RA_continue R' rho ⊢ RA_continue R rho) ->
-   (forall vl rho, ⌜typecheck_environ Delta rho⌝
-                      ∧ RA_return R' vl rho ⊢ RA_return R vl rho) ->
+   (local (typecheck_environ Delta) ∧ P ⊢ P') ->
+   (local (typecheck_environ Delta)
+                      ∧  RA_normal R' ⊢ RA_normal R) ->
+   (local (typecheck_environ Delta)
+                      ∧ RA_break R' ⊢ RA_break R) ->
+   (local (typecheck_environ Delta)
+                      ∧ RA_continue R' ⊢ RA_continue R) ->
+   (forall vl, local (typecheck_environ Delta)
+                      ∧ RA_return R' vl ⊢ RA_return R vl) ->
    semax Espec E Delta P' c R' ->  semax Espec E Delta P c R.
 Proof.
 intros.
@@ -572,7 +581,7 @@ Qed.
 
 Lemma semax_fupd_elim {CS: compspecs}:
  forall E Delta P c R,
-  semax Espec E Delta P c R -> semax Espec E Delta (fun rho => |={E}=> (P rho)) c R.
+  semax Espec E Delta P c R -> semax Espec E Delta (|={E}=> P) c R.
 Proof.
 intros; eapply semax_pre_fupd, H.
 by intros; rewrite bi.and_elim_r.
@@ -592,21 +601,21 @@ Lemma semax_extract_prop:
   forall {CS: compspecs},
   forall E Delta (PP: Prop) (P:assert) c (Q:ret_assert),
            (PP -> semax Espec E Delta P c Q) ->
-           semax Espec E Delta (fun rho => ⌜PP⌝ ∧ P rho) c Q.
+           semax Espec E Delta (⌜PP⌝ ∧ P) c Q.
 Proof.
   intros.
-  eapply semax_pre with (fun rho => ∃ H: PP, P rho).
-  + intros; iIntros "(% & %HPP & ?)"; iExists HPP; auto.
+  eapply semax_pre with (∃ H: PP, P).
+  + intros; iIntros "(? & %HPP & ?)"; iExists HPP; auto.
   + apply extract_exists_pre, H.
 Qed.
 
 Lemma semax_adapt_frame {cs} E Delta c (P P': assert) (Q Q' : ret_assert)
-   (H: forall rho,  ⌜typecheck_environ Delta rho⌝ ∧ (<affine> allp_fun_id E Delta rho ∗ P rho) ⊢
-                   ∃ F: assert, (⌜closed_wrt_modvars c F⌝ ∧ |={E}=> (P' rho ∗ F rho) ∧
-                         ⌜forall rho, ((local (tc_environ Delta) rho) ∧ <affine> allp_fun_id E Delta rho ∗ RA_normal (frame_ret_assert Q' F) rho ⊢ |={E}=> RA_normal Q rho)⌝ ∧
-                         ⌜forall rho, ((local (tc_environ Delta) rho) ∧ <affine> allp_fun_id E Delta rho ∗ RA_break (frame_ret_assert Q' F) rho ⊢ |={E}=> RA_break Q rho)⌝ ∧
-                         ⌜forall rho, ((local (tc_environ Delta) rho) ∧ <affine> allp_fun_id E Delta rho ∗ RA_continue (frame_ret_assert Q' F) rho ⊢ |={E}=> RA_continue Q rho)⌝ ∧
-                         ⌜forall vl rho, ((local (tc_environ Delta) rho) ∧ <affine> allp_fun_id E Delta rho ∗ RA_return (frame_ret_assert Q' F) vl rho ⊢ RA_return Q vl rho)⌝))
+   (H: local (typecheck_environ Delta) ∧ (<affine> allp_fun_id E Delta ∗ P) ⊢
+                   ∃ F: assert, (⌜closed_wrt_modvars c F⌝ ∧ |={E}=> (P' ∗ F) ∧
+                         ⌜local (tc_environ Delta) ∧ <affine> allp_fun_id E Delta ∗ RA_normal (frame_ret_assert Q' F) ⊢ |={E}=> RA_normal Q⌝ ∧
+                         ⌜local (tc_environ Delta) ∧ <affine> allp_fun_id E Delta ∗ RA_break (frame_ret_assert Q' F) ⊢ |={E}=> RA_break Q⌝ ∧
+                         ⌜local (tc_environ Delta) ∧ <affine> allp_fun_id E Delta ∗ RA_continue (frame_ret_assert Q' F) ⊢ |={E}=> RA_continue Q⌝ ∧
+                         ⌜forall vl, local (tc_environ Delta) ∧ <affine> allp_fun_id E Delta ∗ RA_return (frame_ret_assert Q' F) vl ⊢ RA_return Q vl⌝))
    (SEM: semax Espec E Delta P' c Q'):
    semax Espec E Delta P c Q.
 Proof.
@@ -627,12 +636,12 @@ Proof.
 Qed.
 
 Lemma semax_adapt_frame' {cs} E Delta c (P P': assert) (Q Q' : ret_assert)
-   (H: forall rho,  ⌜typecheck_environ Delta rho⌝ ∧ (<affine> allp_fun_id E Delta rho ∗ P rho) ⊢
-                   ∃ F: assert, (⌜closed_wrt_modvars c F⌝ ∧ |={E}=> (P' rho ∗ F rho) ∧
-                         ⌜forall rho, (RA_normal (frame_ret_assert Q' F) rho ⊢ |={E}=> RA_normal Q rho)⌝ ∧
-                         ⌜forall rho, (RA_break (frame_ret_assert Q' F) rho ⊢ |={E}=> RA_break Q rho)⌝ ∧
-                         ⌜forall rho, (RA_continue (frame_ret_assert Q' F) rho ⊢ |={E}=> RA_continue Q rho)⌝ ∧
-                         ⌜forall vl rho, (RA_return (frame_ret_assert Q' F) vl rho ⊢ RA_return Q vl rho)⌝))
+   (H: local (typecheck_environ Delta) ∧ (<affine> allp_fun_id E Delta ∗ P) ⊢
+                   ∃ F: assert, (⌜closed_wrt_modvars c F⌝ ∧ |={E}=> (P' ∗ F) ∧
+                         ⌜RA_normal (frame_ret_assert Q' F) ⊢ |={E}=> RA_normal Q⌝ ∧
+                         ⌜RA_break (frame_ret_assert Q' F) ⊢ |={E}=> RA_break Q⌝ ∧
+                         ⌜RA_continue (frame_ret_assert Q' F) ⊢ |={E}=> RA_continue Q⌝ ∧
+                         ⌜forall vl, RA_return (frame_ret_assert Q' F) vl ⊢ RA_return Q vl⌝))
    (SEM: semax Espec E Delta P' c Q'):
    semax Espec E Delta P c Q.
 Proof.
@@ -644,20 +653,21 @@ Proof.
 Qed.
 
 Lemma semax_adapt {cs} E Delta c (P P': assert) (Q Q' : ret_assert)
-   (H: forall rho,  ⌜typecheck_environ Delta rho⌝ ∧ (<affine> allp_fun_id E Delta rho ∗ P rho) ⊢
-                   (|={E}=> (P' rho) ∧
-                        ⌜forall rho, RA_normal Q' rho ⊢ |={E}=> RA_normal Q rho⌝ ∧
-                        ⌜forall rho, RA_break Q' rho ⊢ |={E}=> RA_break Q rho⌝ ∧
-                        ⌜forall rho, RA_continue Q' rho ⊢ |={E}=> RA_continue Q rho⌝ ∧
-                        ⌜forall vl rho, RA_return Q' vl rho ⊢ RA_return Q vl rho⌝))
+   (H: local (typecheck_environ Delta) ∧ (<affine> allp_fun_id E Delta ∗ P) ⊢
+                   (|={E}=> P' ∧
+                        ⌜RA_normal Q' ⊢ |={E}=> RA_normal Q⌝ ∧
+                        ⌜RA_break Q' ⊢ |={E}=> RA_break Q⌝ ∧
+                        ⌜RA_continue Q' ⊢ |={E}=> RA_continue Q⌝ ∧
+                        ⌜forall vl, RA_return Q' vl ⊢ RA_return Q vl⌝))
    (SEM: semax Espec E Delta P' c Q'):
    semax Espec E Delta P c Q.
 Proof.
-  intros. eapply semax_adapt_frame'; eauto. intros. rewrite H; iIntros "H"; iExists (fun rho => emp).
-  iSplit; first done.
+  intros. eapply semax_adapt_frame'; eauto. intros. rewrite H; iIntros "H"; iExists emp.
+  iSplit.
+  { iPureIntro; monPred.unseal; done. }
   iMod "H" as "($ & %NORM & %BREAK & %CONT & %RET)"; iPureIntro; split; auto.
   destruct Q'; simpl in *.
-  split3; last split; intros; monPred.unseal; rewrite right_id; auto.
+  split3; last split; intros; rewrite right_id; auto.
 Qed.
 
 End mpred.
